\documentclass[11pt]{article}
\usepackage{lineno, blindtext,  enumerate, algorithmic }
\usepackage{amssymb} 
\usepackage{amsthm}
\usepackage{amsmath}
\usepackage{graphicx}
\usepackage{xcolor}
\usepackage{subcaption}

\usepackage{listings}
\usepackage{xcolor}

\usepackage[ruled,vlined,linesnumbered]{algorithm2e}

\usepackage{apacite}
\bibliographystyle{apacite}

\definecolor{codegreen}{rgb}{0,0.6,0}
\definecolor{codegray}{rgb}{0.5,0.5,0.5}
\definecolor{codepurple}{rgb}{0.58,0,0.82}
\definecolor{backcolour}{rgb}{0.95,0.95,0.92}
 
\lstdefinestyle{mystyle}{
    backgroundcolor=\color{backcolour},   
    commentstyle=\color{codegreen},
    keywordstyle=\color{magenta},
    numberstyle=\tiny\color{codegray},
    stringstyle=\color{codepurple},
    basicstyle=\ttfamily\footnotesize,
    breakatwhitespace=false,         
    breaklines=true,                 
    captionpos=b,                    
    keepspaces=true,                 
    numbers=left,                    
    numbersep=5pt,                  
    showspaces=false,                
    showstringspaces=false,
    showtabs=false,                  
    tabsize=2
}
 
\lstset{style=mystyle}

\newcommand{\ans}{\ensuremath{\mathbf{ANS.}\quad}}
% \newcommand{\proof}{\ensuremath{\mathbf{PROOF.}\quad}}
\newcommand{\todo}{{\color{red}TODO}}
\newcommand{\solved}{{\color{green}SOLVED}}
\newcommand{\question}[1]{{\item {\bf #1}}}

\renewcommand{\baselinestretch}{1.0}
\setlength{\oddsidemargin}{0.0in}
\setlength{\evensidemargin}{0.0in}
\setlength{\topmargin}{0.0in}
\setlength{\textheight}{8.5in}
\setlength{\textwidth}{6.5in}
\setlength{\headsep}{0in}
\setlength{\parindent}{0in}
\newcommand{\utwi}[1]{\mbox{\boldmath $ #1$}}
\pagestyle{plain}
\includeonly{}

\newcommand\blfootnote[1]{%
  \begingroup
  \renewcommand\thefootnote{}\footnote{#1}%
  \addtocounter{footnote}{-1}%
  \endgroup
}

\begin{document}

\begin{align*}
    & \frac{dS}{dt} = \beta c \frac{I}{N} \\
    \implies &f := \beta c = \frac{I}{N} \left(\frac{dS}{dt}\right)^{-1}
\end{align*}

\begin{align*}
& R^2 = 1 - \frac{\sum_i (y_{true, i} - y_{pred, i})^2}{\sum_i (y_{true, i} - \bar{y}_{true,i})^2}
\end{align*}


\end{document}